\documentclass{article}

%include agda.fmt

\newcommand{\relation}[1]{\kern1.5pt\mathrel{#1}\kern1pt}
\newcommand{\operator}[1]{\kern-2pt\mathop{#1}\kern-3pt}
\newcommand{\constant}[1]{\texttt{#1}}

%subst varid x = "\textit{" x "}"
%subst conid x = "\textit{" x "}"

%format ( = "\text("
%format ) = "\text)"
%format , = "\text{\,,~}"
%format -> = "\relation{\to}"
%format <-> = "\relation{\leftrightarrow}"
%format \ = "\lambda\kern1pt"
%format (highlight(x)) = "{\color{red}" x "}"
%format (dehighlight(x)) = "{\color[gray]{.9}" x "}"
%format (sub (t)) = "\mkern-\medmuskip_{" t "}"
%format (subst (t) (x)) = "\![\kern.5pt" t "/" x "\kern1.225pt]"
%format (Subst (t) (x)) = "\![\kern.5pt" t "\kern1pt/\kern1pt" x "\kern1.225pt]"
%format SKIP = "\mkern-\medmuskip\kern1pt"
%format PRIME = "\mkern-\medmuskip^\prime"
%format 0 = "\mathsf 0"
%format 1 = "\mathsf 1"
%format 2 = "\mathsf 2"

%format : = "\relation{:}"
%format :: = "\relation{::}"
%format ENTAILS = "\relation{\vdash}\!"
%format MODELS = "\relation{\models}\!"
%format BIND = "\kern-2pt."
%format COPY = "\text{---}"
%format = = "\relation{=}\kern-.75pt"
%format DEFEQ = "\kern-2pt\mathrel{\mathop:}=\kern-2pt"
%format IN = "\kern1.5pt\in\kern-1.5pt"
%format ; = "\text{\,;~}"
%format U = "\kern1pt\mathcal U\kern-.5pt"
%format TIMES = "\operator{\times}"
%format fst = "\constant{fst}"
%format snd = "\constant{snd}"
%format fst' = "\textit{fst}"
%format snd' = "\textit{snd}"
%format PLUS = "\operator{+}"
%format left = "\constant{left}"
%format right = "\constant{right}"
%format case = "\constant{case}"
%format TOP = "\top"
%format unit = "\constant{unit}"
%format BOT = "\bot"
%format absurd = "\constant{absurd}"
%format NEG = "\neg\!"
%format BOOL = "\constant{Bool}"
%format false = "\constant{false}"
%format true = "\constant{true}"
%format Pi' = "\Pi"
%format (Pi (x) (t)) = "\Pi\kern1pt[\kern1pt" x ":\kern-.75pt" t "\kern1.25pt]\kern1.5pt"
%format Sigma' = "\Sigma"
%format (Sigma (x) (t)) = "\Sigma\kern1pt[\kern1pt" x ":\kern-.75pt" t "\kern1.25pt]\kern1.5pt"
%format LEM = "\constant{LEM}"
%format Id = "\constant{Id}"
%format refl = "\constant{refl}"
%format transport = "\constant{transport}"
%format J = "\constant{J}"
%format J' = "J"

%format Nat = "\mathbb N"
%format zero = "\constant{zero}"
%format suc = "\constant{suc}"
%format ind = "\constant{ind}"
%format Gamma = "\Gamma"
%format sigma = "\sigma"

%format * = "\kern-1pt\times\kern-1pt"

%format (sem(t)) = "[\![" t "\kern.75pt]\!]"

%format YCOMB = "\constant{Y}\kern-1.5pt"

\renewcommand{\rule}[1]{\RightLabel{\footnotesize (#1)}}

\usepackage[paperwidth=150cm,paperheight=20cm,margin=2cm]{geometry}
\usepackage{nopageno}

\usepackage{bussproofs}
\EnableBpAbbreviations

\begin{document}

\[
\AXC{}
\rule{V}\UIC{|COPY ENTAILS r : (Pi x A) (Sigma y B) R x y|}
\AXC{}
\rule{V}\UIC{|COPY ENTAILS x : A|}
\rule{$\Pi$E}\BIC{|COPY ENTAILS r x : (Sigma y B) R x y|}
\rule{$\Sigma$EL}\UIC{|COPY , x : A ENTAILS fst (r x) : B|}
\rule{$\to$I}\UIC{|COPY ENTAILS \ x BIND fst (r x) : A -> B|}
\AXC{}
\rule{V}\UIC{|COPY ENTAILS r : (Pi x A) (Sigma y B) R x y|}
\AXC{}
\rule{V}\UIC{|COPY ENTAILS x PRIME : A|}
\rule{$\Pi$E}\BIC{|COPY ENTAILS r x PRIME : (Sigma y B) R x PRIME y|}
\rule{$\Sigma$ER}\UIC{|COPY ENTAILS snd (r x PRIME) : R x PRIME (fst (r x PRIME))|}
\AXC{}
\rule{V}\UIC{|COPY ENTAILS R : A -> B -> U|}
\AXC{}
\rule{V}\UIC{|COPY ENTAILS x PRIME : A|}
\rule{$\to$I}\BIC{|COPY ENTAILS R x PRIME : B -> U|}
\rule{refl}\UIC{|COPY ENTAILS R x PRIME = R x PRIME IN B -> U|}
\AXC{}
\rule{V}\UIC{|COPY ENTAILS r : (Pi x A) (Sigma y B) R x y|}
\AXC{}
\rule{V}\UIC{|COPY ENTAILS x : A|}
\rule{$\Pi$E}\BIC{|COPY ENTAILS r x : (Sigma y B) R x y|}
\rule{$\Sigma$EL}\UIC{|COPY , x : A ENTAILS fst (r x) : B|}
\AXC{}
\rule{V}\UIC{|COPY ENTAILS x PRIME : A|}
\rule{$\to$C}\BIC{|COPY ENTAILS (\ x BIND fst (r x)) x PRIME = fst (r x PRIME) IN B|}
\rule{sym}\UIC{|COPY ENTAILS fst (r x PRIME) = (\ x BIND fst (r x)) x PRIME IN B|}
\rule{cong}\BIC{|COPY ENTAILS R x PRIME (fst (r x PRIME)) = R x PRIME ((\ x BIND fst (r x)) x PRIME) IN U|}
\rule{conv}\BIC{|COPY , x PRIME : A ENTAILS snd (r x PRIME) IN R x PRIME ((\ x BIND fst (r x)) x PRIME)|}
\rule{$\Pi$I}\UIC{|COPY ENTAILS \ x PRIME BIND snd (r x PRIME) : (Pi (x PRIME) A) R x PRIME ((\ x BIND fst (r x)) x PRIME)|}
\rule{$\Sigma$I}\BIC{|COPY , r : (Pi x A) (Sigma y B) R x y ENTAILS ((\ x BIND fst (r x)) , (\ x PRIME BIND snd (r x PRIME))) : (Sigma f (A -> B)) (Pi (x PRIME) A) R x PRIME (f x PRIME)|}
\rule{$\to$I}\UIC{|A : U, B : U, R : A -> B -> U ENTAILS \ r BIND ((\ x BIND fst (r x)) , (\ x PRIME BIND snd (r x PRIME))) : ((Pi x A) (Sigma y B) R x y) -> (Sigma f (A -> B)) (Pi (x PRIME) A) R x PRIME (f x PRIME)|}
\DP \]

\[
\AXC{}
\rule{V}\UIC{|A : U, B : U, R : A -> B -> U , r : (Pi x A) (Sigma y B) R x y , x : A ENTAILS r : (Pi x A) (Sigma y B) R x y|}
\AXC{}
\rule{V}\UIC{|A : U, B : U, R : A -> B -> U , r : (Pi x A) (Sigma y B) R x y , x : A ENTAILS x : A|}
\rule{$\Pi$E}\BIC{|A : U, B : U, R : A -> B -> U , r : (Pi x A) (Sigma y B) R x y , x : A ENTAILS r x : (Sigma y B) R x y|}
\rule{$\Sigma$EL}\UIC{|A : U, B : U, R : A -> B -> U , r : (Pi x A) (Sigma y B) R x y , x : A ENTAILS fst (r x) : B|}
\rule{$\to$I}\UIC{|A : U, B : U, R : A -> B -> U , r : (Pi x A) (Sigma y B) R x y ENTAILS \ x BIND fst (r x) : A -> B|}
\AXC{}
\rule{V}\UIC{|A : U, B : U, R : A -> B -> U , r : (Pi x A) (Sigma y B) R x y , x PRIME : A ENTAILS r : (Pi x A) (Sigma y B) R x y|}
\AXC{}
\rule{V}\UIC{|A : U, B : U, R : A -> B -> U , r : (Pi x A) (Sigma y B) R x y , x PRIME : A ENTAILS x PRIME : A|}
\rule{$\Pi$E}\BIC{|A : U, B : U, R : A -> B -> U , r : (Pi x A) (Sigma y B) R x y , x PRIME : A ENTAILS r x PRIME : (Sigma y B) R x PRIME y|}
\rule{$\Sigma$ER}\UIC{|A : U, B : U, R : A -> B -> U , r : (Pi x A) (Sigma y B) R x y , x PRIME : A ENTAILS snd (r x PRIME) : R x PRIME (fst (r x PRIME))|}
\AXC{}
\rule{V}\UIC{|A : U, B : U, R : A -> B -> U , r : (Pi x A) (Sigma y B) R x y , x PRIME : A ENTAILS R : A -> B -> U|}
\AXC{}
\rule{V}\UIC{|A : U, B : U, R : A -> B -> U , r : (Pi x A) (Sigma y B) R x y , x PRIME : A ENTAILS x PRIME : A|}
\rule{$\to$I}\BIC{|A : U, B : U, R : A -> B -> U , r : (Pi x A) (Sigma y B) R x y , x PRIME : A ENTAILS R x PRIME : B -> U|}
\rule{refl}\UIC{|A : U, B : U, R : A -> B -> U , r : (Pi x A) (Sigma y B) R x y , x PRIME : A ENTAILS R x PRIME = R x PRIME IN B -> U|}
\AXC{}
\rule{V}\UIC{|A : U, B : U, R : A -> B -> U , r : (Pi x A) (Sigma y B) R x y , x PRIME : A , x : A ENTAILS r : (Pi x A) (Sigma y B) R x y|}
\AXC{}
\rule{V}\UIC{|A : U, B : U, R : A -> B -> U , r : (Pi x A) (Sigma y B) R x y , x PRIME : A , x : A ENTAILS x : A|}
\rule{$\Pi$E}\BIC{|A : U, B : U, R : A -> B -> U , r : (Pi x A) (Sigma y B) R x y , x PRIME : A , x : A ENTAILS r x : (Sigma y B) R x y|}
\rule{$\Sigma$EL}\UIC{|A : U, B : U, R : A -> B -> U , r : (Pi x A) (Sigma y B) R x y , x PRIME : A , x : A ENTAILS fst (r x) : B|}
\AXC{}
\rule{V}\UIC{|A : U, B : U, R : A -> B -> U , r : (Pi x A) (Sigma y B) R x y , x PRIME : A ENTAILS x PRIME : A|}
\rule{$\to$C}\BIC{|A : U, B : U, R : A -> B -> U , r : (Pi x A) (Sigma y B) R x y , x PRIME : A ENTAILS (\ x BIND fst (r x)) x PRIME = fst (r x PRIME) IN B|}
\rule{sym}\UIC{|A : U, B : U, R : A -> B -> U , r : (Pi x A) (Sigma y B) R x y , x PRIME : A ENTAILS fst (r x PRIME) = (\ x BIND fst (r x)) x PRIME IN B|}
\rule{cong}\BIC{|A : U, B : U, R : A -> B -> U , r : (Pi x A) (Sigma y B) R x y , x PRIME : A ENTAILS R x PRIME (fst (r x PRIME)) = R x PRIME ((\ x BIND fst (r x)) x PRIME) IN U|}
\rule{conv}\BIC{|A : U, B : U, R : A -> B -> U , r : (Pi x A) (Sigma y B) R x y , x PRIME : A ENTAILS snd (r x PRIME) IN R x PRIME ((\ x BIND fst (r x)) x PRIME)|}
\rule{$\Pi$I}\UIC{|A : U, B : U, R : A -> B -> U , r : (Pi x A) (Sigma y B) R x y ENTAILS \ x PRIME BIND snd (r x PRIME) : (Pi (x PRIME) A) R x PRIME ((\ x BIND fst (r x)) x PRIME)|}
\rule{$\Sigma$I}\BIC{|A : U, B : U, R : A -> B -> U , r : (Pi x A) (Sigma y B) R x y ENTAILS ((\ x BIND fst (r x)) , (\ x PRIME BIND snd (r x PRIME))) : (Sigma f (A -> B)) (Pi (x PRIME) A) R x PRIME (f x PRIME)|}
\rule{$\to$I}\UIC{|A : U, B : U, R : A -> B -> U ENTAILS \ r BIND ((\ x BIND fst (r x)) , (\ x PRIME BIND snd (r x PRIME))) : ((Pi x A) (Sigma y B) R x y) -> (Sigma f (A -> B)) (Pi (x PRIME) A) R x PRIME (f x PRIME)|}
\DP \]

\end{document}